updated to new boogieamp version

gravy/test/out.bpl
@@ -9,18 +9,15 @@ type intArrHeap_type = [ref][int]int;
 const unique $type : Field javaType;
 const unique $alloc : Field bool;
 const unique $null : ref;
-const { :sourceloc "/Users/schaef/git/jar2bpl/jar2bpl_test/regression/false_positives/fp08/FalsePositives08.java",-1,-1,-1,-1 } unique java.lang.Object : javaType extends  complete;
-const { :sourceloc "/Users/schaef/git/jar2bpl/jar2bpl_test/regression/false_positives/fp08/FalsePositives08.java",-1,-1,-1,-1 } unique FalsePositives08 : javaType extends  unique java.lang.Object complete;
-const { :sourceloc "/Users/schaef/git/jar2bpl/jar2bpl_test/regression/false_positives/fp08/FalsePositives08.java",-1,-1,-1,-1 } unique java.io.Serializable : javaType extends  unique java.lang.Object complete;
-const { :sourceloc "/Users/schaef/git/jar2bpl/jar2bpl_test/regression/false_positives/fp08/FalsePositives08.java",-1,-1,-1,-1 } unique java.lang.Throwable : javaType extends  unique java.lang.Object, unique java.io.Serializable complete;
-const { :sourceloc "/Users/schaef/git/jar2bpl/jar2bpl_test/regression/false_positives/fp08/FalsePositives08.java",-1,-1,-1,-1 } unique java.lang.Exception : javaType extends  unique java.lang.Throwable complete;
-const { :sourceloc "/Users/schaef/git/jar2bpl/jar2bpl_test/regression/false_positives/fp08/FalsePositives08.java",-1,-1,-1,-1 } unique java.lang.RuntimeException : javaType extends  unique java.lang.Exception complete;
-const { :sourceloc "/Users/schaef/git/jar2bpl/jar2bpl_test/regression/false_positives/fp08/FalsePositives08.java",-1,-1,-1,-1 } unique java.lang.NullPointerException : javaType extends  unique java.lang.RuntimeException complete;
-const { :sourceloc "/Users/schaef/git/jar2bpl/jar2bpl_test/regression/false_positives/fp08/FalsePositives08.java",-1,-1,-1,-1 } unique java.lang.Comparable : javaType extends  unique java.lang.Object complete;
-const { :sourceloc "/Users/schaef/git/jar2bpl/jar2bpl_test/regression/false_positives/fp08/FalsePositives08.java",-1,-1,-1,-1 } unique java.lang.CharSequence : javaType extends  unique java.lang.Object complete;
-const { :sourceloc "/Users/schaef/git/jar2bpl/jar2bpl_test/regression/false_positives/fp08/FalsePositives08.java",-1,-1,-1,-1 } unique java.lang.String : javaType extends  unique java.lang.Comparable, unique java.lang.CharSequence, unique java.lang.Object, unique java.io.Serializable complete;
-const { :sourceloc "/Users/schaef/git/jar2bpl/jar2bpl_test/regression/false_positives/fp08/FalsePositives08.java",-1,-1,-1,-1 } unique java.lang.IndexOutOfBoundsException : javaType extends  unique java.lang.RuntimeException complete;
-const { :sourceloc "/Users/schaef/git/jar2bpl/jar2bpl_test/regression/false_positives/fp08/FalsePositives08.java",-1,-1,-1,-1 } unique java.lang.ArrayIndexOutOfBoundsException : javaType extends  unique java.lang.IndexOutOfBoundsException complete;
+const { :sourceloc "/Users/schaef/git/jar2bpl/jar2bpl_test/regression/corner_cases/cc01/CornerCases01.java",-1,-1,-1,-1 } unique java.lang.Object : javaType extends  complete;
+const { :sourceloc "/Users/schaef/git/jar2bpl/jar2bpl_test/regression/corner_cases/cc01/CornerCases01.java",-1,-1,-1,-1 } unique CornerCases01 : javaType extends  unique java.lang.Object complete;
+const { :sourceloc "/Users/schaef/git/jar2bpl/jar2bpl_test/regression/corner_cases/cc01/CornerCases01.java",-1,-1,-1,-1 } unique java.io.Serializable : javaType extends  unique java.lang.Object complete;
+const { :sourceloc "/Users/schaef/git/jar2bpl/jar2bpl_test/regression/corner_cases/cc01/CornerCases01.java",-1,-1,-1,-1 } unique java.lang.Throwable : javaType extends  unique java.io.Serializable, unique java.lang.Object complete;
+const { :sourceloc "/Users/schaef/git/jar2bpl/jar2bpl_test/regression/corner_cases/cc01/CornerCases01.java",-1,-1,-1,-1 } unique java.lang.Exception : javaType extends  unique java.lang.Throwable complete;
+const { :sourceloc "/Users/schaef/git/jar2bpl/jar2bpl_test/regression/corner_cases/cc01/CornerCases01.java",-1,-1,-1,-1 } unique java.lang.RuntimeException : javaType extends  unique java.lang.Exception complete;
+const { :sourceloc "/Users/schaef/git/jar2bpl/jar2bpl_test/regression/corner_cases/cc01/CornerCases01.java",-1,-1,-1,-1 } unique java.lang.Iterable : javaType extends  unique java.lang.Object complete;
+const { :sourceloc "/Users/schaef/git/jar2bpl/jar2bpl_test/regression/corner_cases/cc01/CornerCases01.java",-1,-1,-1,-1 } unique java.util.Collection : javaType extends  unique java.lang.Iterable, unique java.lang.Object complete;
+const { :sourceloc "/Users/schaef/git/jar2bpl/jar2bpl_test/regression/corner_cases/cc01/CornerCases01.java",-1,-1,-1,-1 } unique java.util.List : javaType extends  unique java.lang.Object, unique java.util.Collection complete;
 var $heap : $heap_type;
 var $intArrayType : javaType;
 var $charArrayType : javaType;
@@ -33,9 +30,6 @@ var $boolArrHeap : boolArrHeap_type;
 var $refArrHeap : refArrHeap_type;
 var $realArrHeap : realArrHeap_type;
 var $intArrHeap : intArrHeap_type;
-var java.lang.Object$FalsePositives08$constraintsLock234 : Field ref;
-var java.lang.String$lp$$rp$$FalsePositives08$constraints235 : Field ref;
-var java.lang.String$FalsePositives08$constraint236 : Field ref;
 function $arrayType(t:javaType) returns ($ret:javaType);
 function $intToReal(x:int) returns ($ret:real);
 function $intToBool(x:int) returns ($ret:bool) { (if x == 0 then false else true) }
@@ -52,183 +46,516 @@ function $shlInt(x:int, y:int) returns ($ret:int);
 function $ushrInt(x:int, y:int) returns ($ret:int);
 function $shrInt(x:int, y:int) returns ($ret:int);
 axiom (forall t : javaType :: $heap[$null,$type] <: t);
-procedure $new(obj_type:javaType) returns ($obj:ref);    ensures $heap[$obj,$alloc] == true;    ensures $obj != $null;    ensures $heap[$obj,$type] == obj_type;    requires $heap[$obj,$alloc] == false;    
+procedure $new(obj_type:javaType) returns ($obj:ref);    ensures $heap[$obj,$alloc] == true;    requires $heap[$obj,$alloc] == false;    ensures $heap[$obj,$type] == obj_type;        ensures $obj != $null;
 
-procedure java.lang.Object$java.lang.Object$clone$43($this:ref) returns ($other:ref);        ensures $heap[$other,$alloc] == true;    ensures $heap[$other,$type] == $heap[$this,$type];    ensures $other != $null;
+procedure java.lang.Object$java.lang.Object$clone$43($this:ref) returns ($other:ref);        ensures $heap[$other,$type] == $heap[$this,$type];    ensures $heap[$other,$alloc] == true;    ensures $other != $null;
 
 procedure int$java.lang.String$compareTo$87($this:ref, $other:ref) returns ($return:int);    
 
-procedure void$FalsePositives08$fp01$1889($this:ref) returns ($exception:ref);    modifies $refArrHeap, $heap, $arrSizeHeap;
+procedure void$CornerCases01$decideCondition$1889($this:ref, $in_parameter__0:int, $in_parameter__1:int) returns ($exception:ref);    
 
-procedure void$FalsePositives08$$la$init$ra$$1890($this:ref) returns ($exception:ref);    
+procedure void$java.lang.RuntimeException$$la$init$ra$$922($this:ref) returns ($exception:ref);    
+
+procedure int$CornerCases01$decisions$1890($this:ref, $in_parameter__0:int, $in_parameter__1:int) returns ($return:int, $exception:ref);    
+
+procedure int$CornerCases01$getNewIndex$1891($this:ref, $in_parameter__0:int, $in_parameter__1:ref, $in_parameter__2:ref, $in_parameter__3:ref, $in_parameter__4:ref) returns ($return:int, $exception:ref);    modifies $heap;
+
+procedure int$java.util.List$size$152($this:ref) returns ($return:int, $exception:ref);    modifies $heap;
+
+procedure int$CornerCases01$getInt$1892($this:ref, $in_parameter__0:int) returns ($return:int, $exception:ref);    
+
+procedure void$CornerCases01$$la$init$ra$$1893($this:ref) returns ($exception:ref);    
 
 procedure void$java.lang.Object$$la$init$ra$$38($this:ref) returns ($exception:ref);    
 
-implementation void$FalsePositives08$fp01$1889($this:ref) returns ($exception:ref){
+implementation void$CornerCases01$decideCondition$1889($this:ref, $in_parameter__0:int, $in_parameter__1:int) returns ($exception:ref){
     
-var temp$1216 : int;    
-var i7 : int;    
-var temp$610 : ref;    
 var $fakelocal_0 : ref;    
+var temp$04 : ref;    
 var this1 : ref;    
-var temp$812 : ref;    
-var temp$36 : int;    
-var temp$1014 : ref;    
-var temp$25 : int;    
-var temp$1620 : ref;    
-var temp$1418 : ref;    
-var temp$1317 : ref;    
-var temp$48 : ref;    
-var temp$711 : int;    
-var temp$59 : int;    
-var temp$14 : ref;    
-var temp$1721 : ref;    
-var temp$913 : int;    
-var results3 : ref;    
-var temp$1115 : int;    
-var temp$02 : ref;    
-var temp$1519 : int;
-    assume { :sourceloc "/Users/schaef/git/jar2bpl/jar2bpl_test/regression/false_positives/fp08/FalsePositives08.java",-1,-1,-1,-1 } $this != $null;
-    assert { :sourceloc "/Users/schaef/git/jar2bpl/jar2bpl_test/regression/false_positives/fp08/FalsePositives08.java",8,2,19,2 } true;
+var notEqual3 : int;    
+var truthValue2 : int;
+    assume { :sourceloc "/Users/schaef/git/jar2bpl/jar2bpl_test/regression/corner_cases/cc01/CornerCases01.java",-1,-1,-1,-1 } $this != $null;
+    assert { :sourceloc "/Users/schaef/git/jar2bpl/jar2bpl_test/regression/corner_cases/cc01/CornerCases01.java",10,2,25,2 } true;
     this1 := $this;
-    assert { :sourceloc "/Users/schaef/git/jar2bpl/jar2bpl_test/regression/false_positives/fp08/FalsePositives08.java",10,23,10,37 } true;
-    temp$02 := $heap[this1,java.lang.Object$FalsePositives08$constraintsLock234];
-    assert { :sourceloc "/Users/schaef/git/jar2bpl/jar2bpl_test/regression/false_positives/fp08/FalsePositives08.java",10,23,10,37 } true;
-    havoc temp$02, this1, $exception, $heap;
-  block1:
-    assert { :sourceloc "/Users/schaef/git/jar2bpl/jar2bpl_test/regression/false_positives/fp08/FalsePositives08.java",10,23,10,37 } true;
-    assert { :sourceloc "/Users/schaef/git/jar2bpl/jar2bpl_test/regression/false_positives/fp08/FalsePositives08.java",12,28,12,38 } true;
-    temp$14 := $heap[this1,java.lang.String$lp$$rp$$FalsePositives08$constraints235];
-    assert { :sourceloc "/Users/schaef/git/jar2bpl/jar2bpl_test/regression/false_positives/fp08/FalsePositives08.java",12,28,12,38 } true;
-    if (temp$14 != $null) {
-        assert { :sourceloc "/Users/schaef/git/jar2bpl/jar2bpl_test/regression/false_positives/fp08/FalsePositives08.java",12,28,12,38 } true;
-    } else {
-        assert { :noverify } true;
-        call $exception := $new(java.lang.NullPointerException);
-        goto block2;
+    assert { :sourceloc "/Users/schaef/git/jar2bpl/jar2bpl_test/regression/corner_cases/cc01/CornerCases01.java",10,30,10,43 } true;
+    truthValue2 := $in_parameter__0;
+    assert { :sourceloc "/Users/schaef/git/jar2bpl/jar2bpl_test/regression/corner_cases/cc01/CornerCases01.java",10,46,10,61 } true;
+    notEqual3 := $in_parameter__1;
+    assert { :sourceloc "/Users/schaef/git/jar2bpl/jar2bpl_test/regression/corner_cases/cc01/CornerCases01.java",14,7,14,14 } true;
+    if (notEqual3 == 0) {
+        assert { :sourceloc "/Users/schaef/git/jar2bpl/jar2bpl_test/regression/corner_cases/cc01/CornerCases01.java",15,4,15,10 } true;
+        goto block1;
     }
-    temp$25 := $arrSizeHeap[temp$14];
-    assert { :sourceloc "/Users/schaef/git/jar2bpl/jar2bpl_test/regression/false_positives/fp08/FalsePositives08.java",12,28,12,38 } true;
-    temp$36 := temp$25 + 1;
-    assert { :sourceloc "/Users/schaef/git/jar2bpl/jar2bpl_test/regression/false_positives/fp08/FalsePositives08.java",12,28,12,38 } true;
-    call $fakelocal_0 := $new($arrayType(java.lang.String));
-    $arrSizeHeap := $arrSizeHeap[$fakelocal_0 := temp$36];
-    results3 := $fakelocal_0;
-    assert { :sourceloc "/Users/schaef/git/jar2bpl/jar2bpl_test/regression/false_positives/fp08/FalsePositives08.java",13,18,13,26 } true;
-    i7 := 0;
+    assert { :sourceloc "/Users/schaef/git/jar2bpl/jar2bpl_test/regression/corner_cases/cc01/CornerCases01.java",14,7,14,14 } true;
+    goto block2;
+  block2:
+    assert { :sourceloc "/Users/schaef/git/jar2bpl/jar2bpl_test/regression/corner_cases/cc01/CornerCases01.java",14,7,14,14 } true;
+    assert { :sourceloc "/Users/schaef/git/jar2bpl/jar2bpl_test/regression/corner_cases/cc01/CornerCases01.java",14,19,14,33 } true;
+    if (truthValue2 == 0) {
+        assert { :sourceloc "/Users/schaef/git/jar2bpl/jar2bpl_test/regression/corner_cases/cc01/CornerCases01.java",14,19,14,33 } true;
+        goto block3;
+    }
+    assert { :sourceloc "/Users/schaef/git/jar2bpl/jar2bpl_test/regression/corner_cases/cc01/CornerCases01.java",14,19,14,33 } true;
+    goto block1;
+    assert { :sourceloc "/Users/schaef/git/jar2bpl/jar2bpl_test/regression/corner_cases/cc01/CornerCases01.java",14,19,14,33 } true;
+    goto block3;
   block3:
-    assert { :sourceloc "/Users/schaef/git/jar2bpl/jar2bpl_test/regression/false_positives/fp08/FalsePositives08.java",13,18,13,26 } true;
-    assert { :sourceloc "/Users/schaef/git/jar2bpl/jar2bpl_test/regression/false_positives/fp08/FalsePositives08.java",13,33,13,43 } true;
-    temp$48 := $heap[this1,java.lang.String$lp$$rp$$FalsePositives08$constraints235];
-    assert { :sourceloc "/Users/schaef/git/jar2bpl/jar2bpl_test/regression/false_positives/fp08/FalsePositives08.java",13,33,13,43 } true;
-    if (temp$48 != $null) {
-        assert { :sourceloc "/Users/schaef/git/jar2bpl/jar2bpl_test/regression/false_positives/fp08/FalsePositives08.java",13,33,13,43 } true;
-    } else {
-        assert { :noverify } true;
-        call $exception := $new(java.lang.NullPointerException);
-        goto block2;
-    }
-    temp$59 := $arrSizeHeap[temp$48];
-    assert { :sourceloc "/Users/schaef/git/jar2bpl/jar2bpl_test/regression/false_positives/fp08/FalsePositives08.java",13,33,13,43 } true;
-    if (i7 < temp$59) {
-        assert { :sourceloc "/Users/schaef/git/jar2bpl/jar2bpl_test/regression/false_positives/fp08/FalsePositives08.java",13,33,13,43 } true;
+    assert { :sourceloc "/Users/schaef/git/jar2bpl/jar2bpl_test/regression/corner_cases/cc01/CornerCases01.java",14,19,14,33 } true;
+    assert { :sourceloc "/Users/schaef/git/jar2bpl/jar2bpl_test/regression/corner_cases/cc01/CornerCases01.java",15,4,15,10 } true;
+    return;
+  block1:
+    assert { :sourceloc "/Users/schaef/git/jar2bpl/jar2bpl_test/regression/corner_cases/cc01/CornerCases01.java",15,4,15,10 } true;
+    assert { :sourceloc "/Users/schaef/git/jar2bpl/jar2bpl_test/regression/corner_cases/cc01/CornerCases01.java",16,14,16,21 } true;
+    if (notEqual3 == 0) {
+        assert { :sourceloc "/Users/schaef/git/jar2bpl/jar2bpl_test/regression/corner_cases/cc01/CornerCases01.java",18,4,18,10 } true;
         goto block4;
     }
-    assert { :sourceloc "/Users/schaef/git/jar2bpl/jar2bpl_test/regression/false_positives/fp08/FalsePositives08.java",13,33,13,43 } true;
+    assert { :sourceloc "/Users/schaef/git/jar2bpl/jar2bpl_test/regression/corner_cases/cc01/CornerCases01.java",16,14,16,21 } true;
     goto block5;
-  block4:
-    assert { :sourceloc "/Users/schaef/git/jar2bpl/jar2bpl_test/regression/false_positives/fp08/FalsePositives08.java",13,33,13,43 } true;
-    assert { :sourceloc "/Users/schaef/git/jar2bpl/jar2bpl_test/regression/false_positives/fp08/FalsePositives08.java",14,17,14,44 } true;
-    temp$610 := results3;
-    assert { :sourceloc "/Users/schaef/git/jar2bpl/jar2bpl_test/regression/false_positives/fp08/FalsePositives08.java",14,17,14,44 } true;
-    temp$711 := i7;
-    assert { :sourceloc "/Users/schaef/git/jar2bpl/jar2bpl_test/regression/false_positives/fp08/FalsePositives08.java",14,30,14,40 } true;
-    temp$812 := $heap[this1,java.lang.String$lp$$rp$$FalsePositives08$constraints235];
-    assert { :sourceloc "/Users/schaef/git/jar2bpl/jar2bpl_test/regression/false_positives/fp08/FalsePositives08.java",14,30,14,40 } true;
-    temp$913 := i7;
-    assert { :sourceloc "/Users/schaef/git/jar2bpl/jar2bpl_test/regression/false_positives/fp08/FalsePositives08.java",14,30,14,40 } true;
-    if (temp$913 < $arrSizeHeap[temp$812] && temp$913 >= 0) {
-        assert { :sourceloc "/Users/schaef/git/jar2bpl/jar2bpl_test/regression/false_positives/fp08/FalsePositives08.java",14,30,14,40 } true;
-    } else {
-        assert { :noverify } true;
-        call $exception := $new(java.lang.ArrayIndexOutOfBoundsException);
-        goto block2;
-    }
-    temp$1014 := $refArrHeap[temp$812][temp$913];
-    assert { :sourceloc "/Users/schaef/git/jar2bpl/jar2bpl_test/regression/false_positives/fp08/FalsePositives08.java",14,24,14,26 } true;
-    if (temp$711 < $arrSizeHeap[temp$610] && temp$711 >= 0) {
-        assert { :sourceloc "/Users/schaef/git/jar2bpl/jar2bpl_test/regression/false_positives/fp08/FalsePositives08.java",14,24,14,26 } true;
-    } else {
-        assert { :noverify } true;
-        call $exception := $new(java.lang.ArrayIndexOutOfBoundsException);
-        goto block2;
-    }
-    $refArrHeap := $refArrHeap[temp$610 := $refArrHeap[temp$610][temp$711 := temp$1014]];
-    assert { :sourceloc "/Users/schaef/git/jar2bpl/jar2bpl_test/regression/false_positives/fp08/FalsePositives08.java",14,24,14,26 } true;
-    assert { :sourceloc "/Users/schaef/git/jar2bpl/jar2bpl_test/regression/false_positives/fp08/FalsePositives08.java",13,53,13,55 } true;
-    temp$1115 := i7;
-    assert { :sourceloc "/Users/schaef/git/jar2bpl/jar2bpl_test/regression/false_positives/fp08/FalsePositives08.java",13,53,13,53 } true;
-    temp$1216 := temp$1115 + 1;
-    assert { :sourceloc "/Users/schaef/git/jar2bpl/jar2bpl_test/regression/false_positives/fp08/FalsePositives08.java",13,53,13,53 } true;
-    i7 := temp$1216;
-    assert { :sourceloc "/Users/schaef/git/jar2bpl/jar2bpl_test/regression/false_positives/fp08/FalsePositives08.java",13,13,14,44 } true;
-    goto block3;
   block5:
-    assert { :sourceloc "/Users/schaef/git/jar2bpl/jar2bpl_test/regression/false_positives/fp08/FalsePositives08.java",13,13,14,44 } true;
-    assert { :sourceloc "/Users/schaef/git/jar2bpl/jar2bpl_test/regression/false_positives/fp08/FalsePositives08.java",15,4,15,44 } true;
-    temp$1317 := results3;
-    assert { :sourceloc "/Users/schaef/git/jar2bpl/jar2bpl_test/regression/false_positives/fp08/FalsePositives08.java",15,12,15,22 } true;
-    temp$1418 := $heap[this1,java.lang.String$lp$$rp$$FalsePositives08$constraints235];
-    assert { :sourceloc "/Users/schaef/git/jar2bpl/jar2bpl_test/regression/false_positives/fp08/FalsePositives08.java",15,12,15,22 } true;
-    if (temp$1418 != $null) {
-        assert { :sourceloc "/Users/schaef/git/jar2bpl/jar2bpl_test/regression/false_positives/fp08/FalsePositives08.java",15,12,15,22 } true;
-    } else {
-        assert { :noverify } true;
-        call $exception := $new(java.lang.NullPointerException);
-        goto block2;
+    assert { :sourceloc "/Users/schaef/git/jar2bpl/jar2bpl_test/regression/corner_cases/cc01/CornerCases01.java",16,14,16,21 } true;
+    assert { :sourceloc "/Users/schaef/git/jar2bpl/jar2bpl_test/regression/corner_cases/cc01/CornerCases01.java",16,26,16,40 } true;
+    if (truthValue2 == 1) {
+        assert { :sourceloc "/Users/schaef/git/jar2bpl/jar2bpl_test/regression/corner_cases/cc01/CornerCases01.java",16,26,16,40 } true;
+        goto block6;
     }
-    temp$1519 := $arrSizeHeap[temp$1418];
-    assert { :sourceloc "/Users/schaef/git/jar2bpl/jar2bpl_test/regression/false_positives/fp08/FalsePositives08.java",15,34,15,43 } true;
-    temp$1620 := $heap[this1,java.lang.String$FalsePositives08$constraint236];
-    assert { :sourceloc "/Users/schaef/git/jar2bpl/jar2bpl_test/regression/false_positives/fp08/FalsePositives08.java",15,11,15,30 } true;
-    if (temp$1519 < $arrSizeHeap[temp$1317] && temp$1519 >= 0) {
-        assert { :sourceloc "/Users/schaef/git/jar2bpl/jar2bpl_test/regression/false_positives/fp08/FalsePositives08.java",15,11,15,30 } true;
-    } else {
-        assert { :noverify } true;
-        call $exception := $new(java.lang.ArrayIndexOutOfBoundsException);
-        goto block2;
-    }
-    $refArrHeap := $refArrHeap[temp$1317 := $refArrHeap[temp$1317][temp$1519 := temp$1620]];
-    assert { :sourceloc "/Users/schaef/git/jar2bpl/jar2bpl_test/regression/false_positives/fp08/FalsePositives08.java",16,13,16,23 } true;
-    $heap := $heap[this1,java.lang.String$lp$$rp$$FalsePositives08$constraints235 := results3];
-    assert { :sourceloc "/Users/schaef/git/jar2bpl/jar2bpl_test/regression/false_positives/fp08/FalsePositives08.java",10,9,17,9 } true;
-    assert { :sourceloc "/Users/schaef/git/jar2bpl/jar2bpl_test/regression/false_positives/fp08/FalsePositives08.java",10,9,17,9 } true;
+    assert { :sourceloc "/Users/schaef/git/jar2bpl/jar2bpl_test/regression/corner_cases/cc01/CornerCases01.java",16,26,16,40 } true;
+    goto block4;
+    assert { :sourceloc "/Users/schaef/git/jar2bpl/jar2bpl_test/regression/corner_cases/cc01/CornerCases01.java",16,26,16,40 } true;
     goto block6;
-  block2:
-    assert { :sourceloc "/Users/schaef/git/jar2bpl/jar2bpl_test/regression/false_positives/fp08/FalsePositives08.java",10,9,17,9 } true;
-    assert { :sourceloc "/Users/schaef/git/jar2bpl/jar2bpl_test/regression/false_positives/fp08/FalsePositives08.java",10,9,17,9 } true;
-    assume $heap[$exception,$type] <: java.lang.Throwable;
-    temp$1721 := $exception;
-    assert { :sourceloc "/Users/schaef/git/jar2bpl/jar2bpl_test/regression/false_positives/fp08/FalsePositives08.java",10,9,17,9 } true;
-    assert { :sourceloc "/Users/schaef/git/jar2bpl/jar2bpl_test/regression/false_positives/fp08/FalsePositives08.java",10,9,17,9 } true;
-    $exception := temp$1721;
-    goto block2;
   block6:
-    assert { :sourceloc "/Users/schaef/git/jar2bpl/jar2bpl_test/regression/false_positives/fp08/FalsePositives08.java",10,9,17,9 } true;
-    assert { :sourceloc "/Users/schaef/git/jar2bpl/jar2bpl_test/regression/false_positives/fp08/FalsePositives08.java",10,9,17,9 } true;
+    assert { :sourceloc "/Users/schaef/git/jar2bpl/jar2bpl_test/regression/corner_cases/cc01/CornerCases01.java",16,26,16,40 } true;
+    assert { :sourceloc "/Users/schaef/git/jar2bpl/jar2bpl_test/regression/corner_cases/cc01/CornerCases01.java",18,4,18,10 } true;
+    return;
+  block4:
+    assert { :sourceloc "/Users/schaef/git/jar2bpl/jar2bpl_test/regression/corner_cases/cc01/CornerCases01.java",18,4,18,10 } true;
+    assert { :sourceloc "/Users/schaef/git/jar2bpl/jar2bpl_test/regression/corner_cases/cc01/CornerCases01.java",19,15,19,22 } true;
+    if (notEqual3 == 0) {
+        assert { :sourceloc "/Users/schaef/git/jar2bpl/jar2bpl_test/regression/corner_cases/cc01/CornerCases01.java",19,15,19,22 } true;
+        goto block7;
+    }
+    assert { :sourceloc "/Users/schaef/git/jar2bpl/jar2bpl_test/regression/corner_cases/cc01/CornerCases01.java",19,15,19,22 } true;
+    goto block8;
+  block7:
+    assert { :sourceloc "/Users/schaef/git/jar2bpl/jar2bpl_test/regression/corner_cases/cc01/CornerCases01.java",19,15,19,22 } true;
+    assert { :sourceloc "/Users/schaef/git/jar2bpl/jar2bpl_test/regression/corner_cases/cc01/CornerCases01.java",19,27,19,41 } true;
+    if (truthValue2 == 0) {
+        assert { :sourceloc "/Users/schaef/git/jar2bpl/jar2bpl_test/regression/corner_cases/cc01/CornerCases01.java",19,27,19,41 } true;
+        goto block9;
+    }
+    assert { :sourceloc "/Users/schaef/git/jar2bpl/jar2bpl_test/regression/corner_cases/cc01/CornerCases01.java",19,27,19,41 } true;
+    goto block8;
+    assert { :sourceloc "/Users/schaef/git/jar2bpl/jar2bpl_test/regression/corner_cases/cc01/CornerCases01.java",19,27,19,41 } true;
+    goto block9;
+  block9:
+    assert { :sourceloc "/Users/schaef/git/jar2bpl/jar2bpl_test/regression/corner_cases/cc01/CornerCases01.java",19,27,19,41 } true;
+    assert { :sourceloc "/Users/schaef/git/jar2bpl/jar2bpl_test/regression/corner_cases/cc01/CornerCases01.java",20,4,20,10 } true;
+    return;
+  block8:
+    assert { :sourceloc "/Users/schaef/git/jar2bpl/jar2bpl_test/regression/corner_cases/cc01/CornerCases01.java",20,4,20,10 } true;
+    assert { :sourceloc "/Users/schaef/git/jar2bpl/jar2bpl_test/regression/corner_cases/cc01/CornerCases01.java",21,15,21,22 } true;
+    if (notEqual3 == 0) {
+        assert { :sourceloc "/Users/schaef/git/jar2bpl/jar2bpl_test/regression/corner_cases/cc01/CornerCases01.java",21,15,21,22 } true;
+        goto block10;
+    }
+    assert { :sourceloc "/Users/schaef/git/jar2bpl/jar2bpl_test/regression/corner_cases/cc01/CornerCases01.java",21,15,21,22 } true;
+    goto block11;
+  block10:
+    assert { :sourceloc "/Users/schaef/git/jar2bpl/jar2bpl_test/regression/corner_cases/cc01/CornerCases01.java",21,15,21,22 } true;
+    assert { :sourceloc "/Users/schaef/git/jar2bpl/jar2bpl_test/regression/corner_cases/cc01/CornerCases01.java",21,27,21,41 } true;
+    if (truthValue2 == 1) {
+        assert { :sourceloc "/Users/schaef/git/jar2bpl/jar2bpl_test/regression/corner_cases/cc01/CornerCases01.java",21,27,21,41 } true;
+        goto block12;
+    }
+    assert { :sourceloc "/Users/schaef/git/jar2bpl/jar2bpl_test/regression/corner_cases/cc01/CornerCases01.java",21,27,21,41 } true;
+    goto block11;
+    assert { :sourceloc "/Users/schaef/git/jar2bpl/jar2bpl_test/regression/corner_cases/cc01/CornerCases01.java",21,27,21,41 } true;
+    goto block12;
+  block12:
+    assert { :sourceloc "/Users/schaef/git/jar2bpl/jar2bpl_test/regression/corner_cases/cc01/CornerCases01.java",21,27,21,41 } true;
+    assert { :sourceloc "/Users/schaef/git/jar2bpl/jar2bpl_test/regression/corner_cases/cc01/CornerCases01.java",22,4,22,10 } true;
+    return;
+  block11:
+    assert { :sourceloc "/Users/schaef/git/jar2bpl/jar2bpl_test/regression/corner_cases/cc01/CornerCases01.java",22,4,22,10 } true;
+    assert { :sourceloc "/Users/schaef/git/jar2bpl/jar2bpl_test/regression/corner_cases/cc01/CornerCases01.java",24,4,24,32 } true;
+    call $fakelocal_0 := $new(java.lang.RuntimeException);
+    temp$04 := $fakelocal_0;
+    assert { :sourceloc "/Users/schaef/git/jar2bpl/jar2bpl_test/regression/corner_cases/cc01/CornerCases01.java",24,10,24,31 } true;
+    call $exception := void$java.lang.RuntimeException$$la$init$ra$$922(temp$04);
+    assert { :sourceloc "/Users/schaef/git/jar2bpl/jar2bpl_test/regression/corner_cases/cc01/CornerCases01.java",24,10,24,31 } true;
+    $exception := temp$04;
+    return;
+    assert { :sourceloc "/Users/schaef/git/jar2bpl/jar2bpl_test/regression/corner_cases/cc01/CornerCases01.java",24,10,24,31 } true;
     return;
 }
 
 
-implementation void$FalsePositives08$$la$init$ra$$1890($this:ref) returns ($exception:ref){
+implementation int$CornerCases01$decisions$1890($this:ref, $in_parameter__0:int, $in_parameter__1:int) returns ($return:int, $exception:ref){
     
-var this22 : ref;
-    assume { :sourceloc "/Users/schaef/git/jar2bpl/jar2bpl_test/regression/false_positives/fp08/FalsePositives08.java",-1,-1,-1,-1 } $this != $null;
-    assert { :sourceloc "/Users/schaef/git/jar2bpl/jar2bpl_test/regression/false_positives/fp08/FalsePositives08.java",3,-1,-1,-1 } true;
-    this22 := $this;
-    assert { :sourceloc "/Users/schaef/git/jar2bpl/jar2bpl_test/regression/false_positives/fp08/FalsePositives08.java",3,-1,-1,-1 } true;
-    call $exception := void$java.lang.Object$$la$init$ra$$38(this22);
-    assert { :sourceloc "/Users/schaef/git/jar2bpl/jar2bpl_test/regression/false_positives/fp08/FalsePositives08.java",3,-1,-1,-1 } true;
+var uppercheck7 : int;    
+var temp$311 : int;    
+var this5 : ref;    
+var temp$19 : int;    
+var temp$08 : int;    
+var temp$210 : int;    
+var lowercheck6 : int;
+    assume { :sourceloc "/Users/schaef/git/jar2bpl/jar2bpl_test/regression/corner_cases/cc01/CornerCases01.java",-1,-1,-1,-1 } $this != $null;
+    assert { :sourceloc "/Users/schaef/git/jar2bpl/jar2bpl_test/regression/corner_cases/cc01/CornerCases01.java",27,2,32,2 } true;
+    this5 := $this;
+    assert { :sourceloc "/Users/schaef/git/jar2bpl/jar2bpl_test/regression/corner_cases/cc01/CornerCases01.java",27,23,27,40 } true;
+    lowercheck6 := $in_parameter__0;
+    assert { :sourceloc "/Users/schaef/git/jar2bpl/jar2bpl_test/regression/corner_cases/cc01/CornerCases01.java",27,43,27,60 } true;
+    uppercheck7 := $in_parameter__1;
+    assert { :sourceloc "/Users/schaef/git/jar2bpl/jar2bpl_test/regression/corner_cases/cc01/CornerCases01.java",28,13,28,22 } true;
+    if (lowercheck6 == 0) {
+        assert { :sourceloc "/Users/schaef/git/jar2bpl/jar2bpl_test/regression/corner_cases/cc01/CornerCases01.java",28,39,28,47 } true;
+        goto block13;
+    }
+    assert { :sourceloc "/Users/schaef/git/jar2bpl/jar2bpl_test/regression/corner_cases/cc01/CornerCases01.java",28,13,28,22 } true;
+    goto block14;
+  block14:
+    assert { :sourceloc "/Users/schaef/git/jar2bpl/jar2bpl_test/regression/corner_cases/cc01/CornerCases01.java",28,13,28,22 } true;
+    assert { :sourceloc "/Users/schaef/git/jar2bpl/jar2bpl_test/regression/corner_cases/cc01/CornerCases01.java",28,27,28,36 } true;
+    if (uppercheck7 == 0) {
+        assert { :sourceloc "/Users/schaef/git/jar2bpl/jar2bpl_test/regression/corner_cases/cc01/CornerCases01.java",28,39,28,47 } true;
+        goto block13;
+    }
+    assert { :sourceloc "/Users/schaef/git/jar2bpl/jar2bpl_test/regression/corner_cases/cc01/CornerCases01.java",28,27,28,36 } true;
+    goto block15;
+    assert { :sourceloc "/Users/schaef/git/jar2bpl/jar2bpl_test/regression/corner_cases/cc01/CornerCases01.java",28,27,28,36 } true;
+    goto block15;
+  block15:
+    assert { :sourceloc "/Users/schaef/git/jar2bpl/jar2bpl_test/regression/corner_cases/cc01/CornerCases01.java",28,27,28,36 } true;
+    assert { :sourceloc "/Users/schaef/git/jar2bpl/jar2bpl_test/regression/corner_cases/cc01/CornerCases01.java",28,27,28,36 } true;
+    temp$08 := 0;
+    assert { :sourceloc "/Users/schaef/git/jar2bpl/jar2bpl_test/regression/corner_cases/cc01/CornerCases01.java",28,39,28,47 } true;
+    $return := temp$08;
+    return;
+  block13:
+    assert { :sourceloc "/Users/schaef/git/jar2bpl/jar2bpl_test/regression/corner_cases/cc01/CornerCases01.java",28,39,28,47 } true;
+    assert { :sourceloc "/Users/schaef/git/jar2bpl/jar2bpl_test/regression/corner_cases/cc01/CornerCases01.java",29,18,29,27 } true;
+    if (lowercheck6 == 0) {
+        assert { :sourceloc "/Users/schaef/git/jar2bpl/jar2bpl_test/regression/corner_cases/cc01/CornerCases01.java",29,45,29,53 } true;
+        goto block16;
+    }
+    assert { :sourceloc "/Users/schaef/git/jar2bpl/jar2bpl_test/regression/corner_cases/cc01/CornerCases01.java",29,18,29,27 } true;
+    goto block17;
+  block17:
+    assert { :sourceloc "/Users/schaef/git/jar2bpl/jar2bpl_test/regression/corner_cases/cc01/CornerCases01.java",29,18,29,27 } true;
+    assert { :sourceloc "/Users/schaef/git/jar2bpl/jar2bpl_test/regression/corner_cases/cc01/CornerCases01.java",29,33,29,42 } true;
+    if (uppercheck7 == 0) {
+        assert { :sourceloc "/Users/schaef/git/jar2bpl/jar2bpl_test/regression/corner_cases/cc01/CornerCases01.java",29,33,29,42 } true;
+        goto block18;
+    }
+    assert { :sourceloc "/Users/schaef/git/jar2bpl/jar2bpl_test/regression/corner_cases/cc01/CornerCases01.java",29,33,29,42 } true;
+    goto block16;
+    assert { :sourceloc "/Users/schaef/git/jar2bpl/jar2bpl_test/regression/corner_cases/cc01/CornerCases01.java",29,33,29,42 } true;
+    goto block18;
+  block18:
+    assert { :sourceloc "/Users/schaef/git/jar2bpl/jar2bpl_test/regression/corner_cases/cc01/CornerCases01.java",29,33,29,42 } true;
+    assert { :sourceloc "/Users/schaef/git/jar2bpl/jar2bpl_test/regression/corner_cases/cc01/CornerCases01.java",29,33,29,42 } true;
+    temp$19 := 1;
+    assert { :sourceloc "/Users/schaef/git/jar2bpl/jar2bpl_test/regression/corner_cases/cc01/CornerCases01.java",29,45,29,53 } true;
+    $return := temp$19;
+    return;
+  block16:
+    assert { :sourceloc "/Users/schaef/git/jar2bpl/jar2bpl_test/regression/corner_cases/cc01/CornerCases01.java",29,45,29,53 } true;
+    assert { :sourceloc "/Users/schaef/git/jar2bpl/jar2bpl_test/regression/corner_cases/cc01/CornerCases01.java",30,19,30,28 } true;
+    if (lowercheck6 == 0) {
+        assert { :sourceloc "/Users/schaef/git/jar2bpl/jar2bpl_test/regression/corner_cases/cc01/CornerCases01.java",30,19,30,28 } true;
+        goto block19;
+    }
+    assert { :sourceloc "/Users/schaef/git/jar2bpl/jar2bpl_test/regression/corner_cases/cc01/CornerCases01.java",30,19,30,28 } true;
+    goto block20;
+  block19:
+    assert { :sourceloc "/Users/schaef/git/jar2bpl/jar2bpl_test/regression/corner_cases/cc01/CornerCases01.java",30,19,30,28 } true;
+    assert { :sourceloc "/Users/schaef/git/jar2bpl/jar2bpl_test/regression/corner_cases/cc01/CornerCases01.java",30,33,30,42 } true;
+    if (uppercheck7 == 0) {
+        assert { :sourceloc "/Users/schaef/git/jar2bpl/jar2bpl_test/regression/corner_cases/cc01/CornerCases01.java",30,45,30,53 } true;
+        goto block20;
+    }
+    assert { :sourceloc "/Users/schaef/git/jar2bpl/jar2bpl_test/regression/corner_cases/cc01/CornerCases01.java",30,33,30,42 } true;
+    goto block21;
+    assert { :sourceloc "/Users/schaef/git/jar2bpl/jar2bpl_test/regression/corner_cases/cc01/CornerCases01.java",30,33,30,42 } true;
+    goto block21;
+  block21:
+    assert { :sourceloc "/Users/schaef/git/jar2bpl/jar2bpl_test/regression/corner_cases/cc01/CornerCases01.java",30,33,30,42 } true;
+    assert { :sourceloc "/Users/schaef/git/jar2bpl/jar2bpl_test/regression/corner_cases/cc01/CornerCases01.java",30,33,30,42 } true;
+    temp$210 := 2;
+    assert { :sourceloc "/Users/schaef/git/jar2bpl/jar2bpl_test/regression/corner_cases/cc01/CornerCases01.java",30,45,30,53 } true;
+    $return := temp$210;
+    return;
+  block20:
+    assert { :sourceloc "/Users/schaef/git/jar2bpl/jar2bpl_test/regression/corner_cases/cc01/CornerCases01.java",30,45,30,53 } true;
+    assert { :sourceloc "/Users/schaef/git/jar2bpl/jar2bpl_test/regression/corner_cases/cc01/CornerCases01.java",30,45,30,53 } true;
+    temp$311 := 3;
+    assert { :sourceloc "/Users/schaef/git/jar2bpl/jar2bpl_test/regression/corner_cases/cc01/CornerCases01.java",31,14,31,22 } true;
+    $return := temp$311;
+    return;
+}
+
+
+implementation int$CornerCases01$getNewIndex$1891($this:ref, $in_parameter__0:int, $in_parameter__1:ref, $in_parameter__2:ref, $in_parameter__3:ref, $in_parameter__4:ref) returns ($return:int, $exception:ref){
+    
+var temp$1030 : int;    
+var temp$019 : int;    
+var rand27 : int;    
+var chars15 : ref;    
+var temp$221 : int;    
+var temp$423 : int;    
+var max18 : int;    
+var temp$828 : int;    
+var temp$524 : int;    
+var temp$120 : int;    
+var booleans17 : ref;    
+var temp$625 : int;    
+var index13 : int;    
+var ints14 : ref;    
+var temp$929 : int;    
+var this12 : ref;    
+var temp$1131 : int;    
+var bytes16 : ref;    
+var temp$726 : int;    
+var temp$1232 : int;    
+var temp$322 : int;
+    assume { :sourceloc "/Users/schaef/git/jar2bpl/jar2bpl_test/regression/corner_cases/cc01/CornerCases01.java",-1,-1,-1,-1 } $this != $null;
+    assume $heap[$in_parameter__2,$type] <: java.util.List;
+    assume $heap[$in_parameter__1,$type] <: java.util.List;
+    assume $heap[$in_parameter__4,$type] <: java.util.List;
+    assume $heap[$in_parameter__3,$type] <: java.util.List;
+    assert { :sourceloc "/Users/schaef/git/jar2bpl/jar2bpl_test/regression/corner_cases/cc01/CornerCases01.java",35,2,57,5 } true;
+    this12 := $this;
+    assert { :sourceloc "/Users/schaef/git/jar2bpl/jar2bpl_test/regression/corner_cases/cc01/CornerCases01.java",35,25,35,33 } true;
+    index13 := $in_parameter__0;
+    assert { :sourceloc "/Users/schaef/git/jar2bpl/jar2bpl_test/regression/corner_cases/cc01/CornerCases01.java",35,36,35,52 } true;
+    ints14 := $in_parameter__1;
+    assert { :sourceloc "/Users/schaef/git/jar2bpl/jar2bpl_test/regression/corner_cases/cc01/CornerCases01.java",35,55,35,72 } true;
+    chars15 := $in_parameter__2;
+    assert { :sourceloc "/Users/schaef/git/jar2bpl/jar2bpl_test/regression/corner_cases/cc01/CornerCases01.java",36,4,36,21 } true;
+    bytes16 := $in_parameter__3;
+    assert { :sourceloc "/Users/schaef/git/jar2bpl/jar2bpl_test/regression/corner_cases/cc01/CornerCases01.java",36,24,36,44 } true;
+    booleans17 := $in_parameter__4;
+    assert { :sourceloc "/Users/schaef/git/jar2bpl/jar2bpl_test/regression/corner_cases/cc01/CornerCases01.java",37,7,37,18 } true;
+    max18 := 0;
+    assert { :sourceloc "/Users/schaef/git/jar2bpl/jar2bpl_test/regression/corner_cases/cc01/CornerCases01.java",38,11,38,29 } true;
+    assert { :sourceloc "/Users/schaef/git/jar2bpl/jar2bpl_test/regression/corner_cases/cc01/CornerCases01.java",38,11,38,29 } booleans17 != $null;
+    call temp$019, $exception := int$java.util.List$size$152(booleans17);
+    assert { :sourceloc "/Users/schaef/git/jar2bpl/jar2bpl_test/regression/corner_cases/cc01/CornerCases01.java",38,11,38,29 } true;
+    if (temp$019 > 0) {
+        assert { :sourceloc "/Users/schaef/git/jar2bpl/jar2bpl_test/regression/corner_cases/cc01/CornerCases01.java",38,11,38,29 } true;
+        goto block22;
+    }
+    assert { :sourceloc "/Users/schaef/git/jar2bpl/jar2bpl_test/regression/corner_cases/cc01/CornerCases01.java",38,11,38,29 } true;
+    goto block23;
+  block22:
+    assert { :sourceloc "/Users/schaef/git/jar2bpl/jar2bpl_test/regression/corner_cases/cc01/CornerCases01.java",38,11,38,29 } true;
+    assert { :sourceloc "/Users/schaef/git/jar2bpl/jar2bpl_test/regression/corner_cases/cc01/CornerCases01.java",38,34,38,43 } true;
+    if (index13 < 63) {
+        assert { :sourceloc "/Users/schaef/git/jar2bpl/jar2bpl_test/regression/corner_cases/cc01/CornerCases01.java",38,34,38,43 } true;
+        goto block24;
+    }
+    assert { :sourceloc "/Users/schaef/git/jar2bpl/jar2bpl_test/regression/corner_cases/cc01/CornerCases01.java",38,34,38,43 } true;
+    goto block23;
+    assert { :sourceloc "/Users/schaef/git/jar2bpl/jar2bpl_test/regression/corner_cases/cc01/CornerCases01.java",38,34,38,43 } true;
+    goto block24;
+  block24:
+    assert { :sourceloc "/Users/schaef/git/jar2bpl/jar2bpl_test/regression/corner_cases/cc01/CornerCases01.java",38,34,38,43 } true;
+    assert { :sourceloc "/Users/schaef/git/jar2bpl/jar2bpl_test/regression/corner_cases/cc01/CornerCases01.java",39,9,39,11 } true;
+    temp$120 := 64;
+    assert { :sourceloc "/Users/schaef/git/jar2bpl/jar2bpl_test/regression/corner_cases/cc01/CornerCases01.java",39,9,39,11 } true;
+    max18 := temp$120;
+    assert { :sourceloc "/Users/schaef/git/jar2bpl/jar2bpl_test/regression/corner_cases/cc01/CornerCases01.java",38,7,45,17 } true;
+    goto block25;
+  block23:
+    assert { :sourceloc "/Users/schaef/git/jar2bpl/jar2bpl_test/regression/corner_cases/cc01/CornerCases01.java",38,7,45,17 } true;
+    assert { :sourceloc "/Users/schaef/git/jar2bpl/jar2bpl_test/regression/corner_cases/cc01/CornerCases01.java",40,16,40,31 } true;
+    assert { :sourceloc "/Users/schaef/git/jar2bpl/jar2bpl_test/regression/corner_cases/cc01/CornerCases01.java",40,16,40,31 } bytes16 != $null;
+    call temp$221, $exception := int$java.util.List$size$152(bytes16);
+    assert { :sourceloc "/Users/schaef/git/jar2bpl/jar2bpl_test/regression/corner_cases/cc01/CornerCases01.java",40,16,40,31 } true;
+    if (temp$221 > 0) {
+        assert { :sourceloc "/Users/schaef/git/jar2bpl/jar2bpl_test/regression/corner_cases/cc01/CornerCases01.java",40,16,40,31 } true;
+        goto block26;
+    }
+    assert { :sourceloc "/Users/schaef/git/jar2bpl/jar2bpl_test/regression/corner_cases/cc01/CornerCases01.java",40,16,40,31 } true;
+    goto block27;
+  block26:
+    assert { :sourceloc "/Users/schaef/git/jar2bpl/jar2bpl_test/regression/corner_cases/cc01/CornerCases01.java",40,16,40,31 } true;
+    assert { :sourceloc "/Users/schaef/git/jar2bpl/jar2bpl_test/regression/corner_cases/cc01/CornerCases01.java",40,36,40,45 } true;
+    if (index13 < 56) {
+        assert { :sourceloc "/Users/schaef/git/jar2bpl/jar2bpl_test/regression/corner_cases/cc01/CornerCases01.java",40,36,40,45 } true;
+        goto block28;
+    }
+    assert { :sourceloc "/Users/schaef/git/jar2bpl/jar2bpl_test/regression/corner_cases/cc01/CornerCases01.java",40,36,40,45 } true;
+    goto block27;
+    assert { :sourceloc "/Users/schaef/git/jar2bpl/jar2bpl_test/regression/corner_cases/cc01/CornerCases01.java",40,36,40,45 } true;
+    goto block28;
+  block28:
+    assert { :sourceloc "/Users/schaef/git/jar2bpl/jar2bpl_test/regression/corner_cases/cc01/CornerCases01.java",40,36,40,45 } true;
+    assert { :sourceloc "/Users/schaef/git/jar2bpl/jar2bpl_test/regression/corner_cases/cc01/CornerCases01.java",41,9,41,11 } true;
+    temp$322 := 57;
+    assert { :sourceloc "/Users/schaef/git/jar2bpl/jar2bpl_test/regression/corner_cases/cc01/CornerCases01.java",41,9,41,11 } true;
+    max18 := temp$322;
+    assert { :sourceloc "/Users/schaef/git/jar2bpl/jar2bpl_test/regression/corner_cases/cc01/CornerCases01.java",40,12,45,17 } true;
+    goto block29;
+  block27:
+    assert { :sourceloc "/Users/schaef/git/jar2bpl/jar2bpl_test/regression/corner_cases/cc01/CornerCases01.java",40,12,45,17 } true;
+    assert { :sourceloc "/Users/schaef/git/jar2bpl/jar2bpl_test/regression/corner_cases/cc01/CornerCases01.java",42,16,42,31 } true;
+    assert { :sourceloc "/Users/schaef/git/jar2bpl/jar2bpl_test/regression/corner_cases/cc01/CornerCases01.java",42,16,42,31 } chars15 != $null;
+    call temp$423, $exception := int$java.util.List$size$152(chars15);
+    assert { :sourceloc "/Users/schaef/git/jar2bpl/jar2bpl_test/regression/corner_cases/cc01/CornerCases01.java",42,16,42,31 } true;
+    if (temp$423 > 0) {
+        assert { :sourceloc "/Users/schaef/git/jar2bpl/jar2bpl_test/regression/corner_cases/cc01/CornerCases01.java",42,16,42,31 } true;
+        goto block30;
+    }
+    assert { :sourceloc "/Users/schaef/git/jar2bpl/jar2bpl_test/regression/corner_cases/cc01/CornerCases01.java",42,16,42,31 } true;
+    goto block31;
+  block30:
+    assert { :sourceloc "/Users/schaef/git/jar2bpl/jar2bpl_test/regression/corner_cases/cc01/CornerCases01.java",42,16,42,31 } true;
+    assert { :sourceloc "/Users/schaef/git/jar2bpl/jar2bpl_test/regression/corner_cases/cc01/CornerCases01.java",42,36,42,45 } true;
+    if (index13 < 48) {
+        assert { :sourceloc "/Users/schaef/git/jar2bpl/jar2bpl_test/regression/corner_cases/cc01/CornerCases01.java",42,36,42,45 } true;
+        goto block32;
+    }
+    assert { :sourceloc "/Users/schaef/git/jar2bpl/jar2bpl_test/regression/corner_cases/cc01/CornerCases01.java",42,36,42,45 } true;
+    goto block31;
+    assert { :sourceloc "/Users/schaef/git/jar2bpl/jar2bpl_test/regression/corner_cases/cc01/CornerCases01.java",42,36,42,45 } true;
+    goto block32;
+  block32:
+    assert { :sourceloc "/Users/schaef/git/jar2bpl/jar2bpl_test/regression/corner_cases/cc01/CornerCases01.java",42,36,42,45 } true;
+    assert { :sourceloc "/Users/schaef/git/jar2bpl/jar2bpl_test/regression/corner_cases/cc01/CornerCases01.java",43,9,43,11 } true;
+    temp$524 := 49;
+    assert { :sourceloc "/Users/schaef/git/jar2bpl/jar2bpl_test/regression/corner_cases/cc01/CornerCases01.java",43,9,43,11 } true;
+    max18 := temp$524;
+    assert { :sourceloc "/Users/schaef/git/jar2bpl/jar2bpl_test/regression/corner_cases/cc01/CornerCases01.java",42,12,45,17 } true;
+    goto block33;
+  block31:
+    assert { :sourceloc "/Users/schaef/git/jar2bpl/jar2bpl_test/regression/corner_cases/cc01/CornerCases01.java",42,12,45,17 } true;
+    assert { :sourceloc "/Users/schaef/git/jar2bpl/jar2bpl_test/regression/corner_cases/cc01/CornerCases01.java",44,16,44,30 } true;
+    assert { :sourceloc "/Users/schaef/git/jar2bpl/jar2bpl_test/regression/corner_cases/cc01/CornerCases01.java",44,16,44,30 } ints14 != $null;
+    call temp$625, $exception := int$java.util.List$size$152(ints14);
+    assert { :sourceloc "/Users/schaef/git/jar2bpl/jar2bpl_test/regression/corner_cases/cc01/CornerCases01.java",44,16,44,30 } true;
+    if (temp$625 > 0) {
+        assert { :sourceloc "/Users/schaef/git/jar2bpl/jar2bpl_test/regression/corner_cases/cc01/CornerCases01.java",44,16,44,30 } true;
+        goto block34;
+    }
+    assert { :sourceloc "/Users/schaef/git/jar2bpl/jar2bpl_test/regression/corner_cases/cc01/CornerCases01.java",44,16,44,30 } true;
+    goto block35;
+  block34:
+    assert { :sourceloc "/Users/schaef/git/jar2bpl/jar2bpl_test/regression/corner_cases/cc01/CornerCases01.java",44,16,44,30 } true;
+    assert { :sourceloc "/Users/schaef/git/jar2bpl/jar2bpl_test/regression/corner_cases/cc01/CornerCases01.java",44,35,44,44 } true;
+    if (index13 < 32) {
+        assert { :sourceloc "/Users/schaef/git/jar2bpl/jar2bpl_test/regression/corner_cases/cc01/CornerCases01.java",44,35,44,44 } true;
+        goto block36;
+    }
+    assert { :sourceloc "/Users/schaef/git/jar2bpl/jar2bpl_test/regression/corner_cases/cc01/CornerCases01.java",44,35,44,44 } true;
+    goto block35;
+    assert { :sourceloc "/Users/schaef/git/jar2bpl/jar2bpl_test/regression/corner_cases/cc01/CornerCases01.java",44,35,44,44 } true;
+    goto block36;
+  block36:
+    assert { :sourceloc "/Users/schaef/git/jar2bpl/jar2bpl_test/regression/corner_cases/cc01/CornerCases01.java",44,35,44,44 } true;
+    assert { :sourceloc "/Users/schaef/git/jar2bpl/jar2bpl_test/regression/corner_cases/cc01/CornerCases01.java",45,9,45,11 } true;
+    temp$726 := 33;
+    assert { :sourceloc "/Users/schaef/git/jar2bpl/jar2bpl_test/regression/corner_cases/cc01/CornerCases01.java",45,9,45,11 } true;
+    max18 := temp$726;
+  block35:
+    assert { :sourceloc "/Users/schaef/git/jar2bpl/jar2bpl_test/regression/corner_cases/cc01/CornerCases01.java",45,9,45,11 } true;
+  block33:
+    assert { :sourceloc "/Users/schaef/git/jar2bpl/jar2bpl_test/regression/corner_cases/cc01/CornerCases01.java",45,9,45,11 } true;
+  block29:
+    assert { :sourceloc "/Users/schaef/git/jar2bpl/jar2bpl_test/regression/corner_cases/cc01/CornerCases01.java",45,9,45,11 } true;
+  block25:
+    assert { :sourceloc "/Users/schaef/git/jar2bpl/jar2bpl_test/regression/corner_cases/cc01/CornerCases01.java",45,9,45,11 } true;
+    assert { :sourceloc "/Users/schaef/git/jar2bpl/jar2bpl_test/regression/corner_cases/cc01/CornerCases01.java",47,11,47,18 } true;
+    if (max18 != 0) {
+        assert { :sourceloc "/Users/schaef/git/jar2bpl/jar2bpl_test/regression/corner_cases/cc01/CornerCases01.java",47,11,47,18 } true;
+        goto block37;
+    }
+    assert { :sourceloc "/Users/schaef/git/jar2bpl/jar2bpl_test/regression/corner_cases/cc01/CornerCases01.java",47,11,47,18 } true;
+    goto block38;
+  block37:
+    assert { :sourceloc "/Users/schaef/git/jar2bpl/jar2bpl_test/regression/corner_cases/cc01/CornerCases01.java",47,11,47,18 } true;
+    assert { :sourceloc "/Users/schaef/git/jar2bpl/jar2bpl_test/regression/corner_cases/cc01/CornerCases01.java",48,20,48,28 } true;
+    call temp$828, $exception := int$CornerCases01$getInt$1892(this12, 4);
+    assert { :sourceloc "/Users/schaef/git/jar2bpl/jar2bpl_test/regression/corner_cases/cc01/CornerCases01.java",48,20,48,28 } true;
+    rand27 := temp$828;
+    assert { :sourceloc "/Users/schaef/git/jar2bpl/jar2bpl_test/regression/corner_cases/cc01/CornerCases01.java",49,9,49,26 } true;
+    temp$929 := max18 - index13;
+    assert { :sourceloc "/Users/schaef/git/jar2bpl/jar2bpl_test/regression/corner_cases/cc01/CornerCases01.java",49,9,49,11 } true;
+    max18 := temp$929;
+    assert { :sourceloc "/Users/schaef/git/jar2bpl/jar2bpl_test/regression/corner_cases/cc01/CornerCases01.java",50,13,50,22 } true;
+    if (max18 > rand27) {
+        assert { :sourceloc "/Users/schaef/git/jar2bpl/jar2bpl_test/regression/corner_cases/cc01/CornerCases01.java",50,13,50,22 } true;
+        goto block39;
+    }
+    assert { :sourceloc "/Users/schaef/git/jar2bpl/jar2bpl_test/regression/corner_cases/cc01/CornerCases01.java",50,13,50,22 } true;
+    goto block40;
+  block39:
+    assert { :sourceloc "/Users/schaef/git/jar2bpl/jar2bpl_test/regression/corner_cases/cc01/CornerCases01.java",50,13,50,22 } true;
+    assert { :sourceloc "/Users/schaef/git/jar2bpl/jar2bpl_test/regression/corner_cases/cc01/CornerCases01.java",51,11,51,13 } true;
+    max18 := rand27;
+    assert { :sourceloc "/Users/schaef/git/jar2bpl/jar2bpl_test/regression/corner_cases/cc01/CornerCases01.java",50,9,53,28 } true;
+    goto block41;
+  block40:
+    assert { :sourceloc "/Users/schaef/git/jar2bpl/jar2bpl_test/regression/corner_cases/cc01/CornerCases01.java",50,9,53,28 } true;
+    assert { :sourceloc "/Users/schaef/git/jar2bpl/jar2bpl_test/regression/corner_cases/cc01/CornerCases01.java",52,18,52,25 } true;
+    if (max18 != 1) {
+        assert { :sourceloc "/Users/schaef/git/jar2bpl/jar2bpl_test/regression/corner_cases/cc01/CornerCases01.java",52,18,52,25 } true;
+        goto block42;
+    }
+    assert { :sourceloc "/Users/schaef/git/jar2bpl/jar2bpl_test/regression/corner_cases/cc01/CornerCases01.java",52,18,52,25 } true;
+    goto block43;
+  block42:
+    assert { :sourceloc "/Users/schaef/git/jar2bpl/jar2bpl_test/regression/corner_cases/cc01/CornerCases01.java",52,18,52,25 } true;
+    assert { :sourceloc "/Users/schaef/git/jar2bpl/jar2bpl_test/regression/corner_cases/cc01/CornerCases01.java",53,17,53,27 } true;
+    call temp$1030, $exception := int$CornerCases01$getInt$1892(this12, max18);
+    assert { :sourceloc "/Users/schaef/git/jar2bpl/jar2bpl_test/regression/corner_cases/cc01/CornerCases01.java",53,11,53,13 } true;
+    max18 := temp$1030;
+  block43:
+    assert { :sourceloc "/Users/schaef/git/jar2bpl/jar2bpl_test/regression/corner_cases/cc01/CornerCases01.java",53,11,53,13 } true;
+  block41:
+    assert { :sourceloc "/Users/schaef/git/jar2bpl/jar2bpl_test/regression/corner_cases/cc01/CornerCases01.java",53,11,53,13 } true;
+    assert { :sourceloc "/Users/schaef/git/jar2bpl/jar2bpl_test/regression/corner_cases/cc01/CornerCases01.java",54,9,54,19 } true;
+    temp$1131 := index13;
+    assert { :sourceloc "/Users/schaef/git/jar2bpl/jar2bpl_test/regression/corner_cases/cc01/CornerCases01.java",54,9,54,19 } true;
+    temp$1232 := temp$1131 + max18;
+    assert { :sourceloc "/Users/schaef/git/jar2bpl/jar2bpl_test/regression/corner_cases/cc01/CornerCases01.java",54,9,54,13 } true;
+    index13 := temp$1232;
+  block38:
+    assert { :sourceloc "/Users/schaef/git/jar2bpl/jar2bpl_test/regression/corner_cases/cc01/CornerCases01.java",54,9,54,13 } true;
+    assert { :sourceloc "/Users/schaef/git/jar2bpl/jar2bpl_test/regression/corner_cases/cc01/CornerCases01.java",56,7,56,19 } true;
+    $return := index13;
+    return;
+}
+
+
+implementation int$CornerCases01$getInt$1892($this:ref, $in_parameter__0:int) returns ($return:int, $exception:ref){
+    
+var i34 : int;    
+var this33 : ref;    
+var temp$035 : int;
+    assume { :sourceloc "/Users/schaef/git/jar2bpl/jar2bpl_test/regression/corner_cases/cc01/CornerCases01.java",-1,-1,-1,-1 } $this != $null;
+    assert { :sourceloc "/Users/schaef/git/jar2bpl/jar2bpl_test/regression/corner_cases/cc01/CornerCases01.java",59,2,62,2 } true;
+    this33 := $this;
+    assert { :sourceloc "/Users/schaef/git/jar2bpl/jar2bpl_test/regression/corner_cases/cc01/CornerCases01.java",59,21,59,25 } true;
+    i34 := $in_parameter__0;
+    assert { :sourceloc "/Users/schaef/git/jar2bpl/jar2bpl_test/regression/corner_cases/cc01/CornerCases01.java",59,21,59,25 } true;
+    temp$035 := 0;
+    assert { :sourceloc "/Users/schaef/git/jar2bpl/jar2bpl_test/regression/corner_cases/cc01/CornerCases01.java",61,3,61,11 } true;
+    $return := temp$035;
+    return;
+}
+
+
+implementation void$CornerCases01$$la$init$ra$$1893($this:ref) returns ($exception:ref){
+    
+var this36 : ref;
+    assume { :sourceloc "/Users/schaef/git/jar2bpl/jar2bpl_test/regression/corner_cases/cc01/CornerCases01.java",-1,-1,-1,-1 } $this != $null;
+    assert { :sourceloc "/Users/schaef/git/jar2bpl/jar2bpl_test/regression/corner_cases/cc01/CornerCases01.java",5,-1,-1,-1 } true;
+    this36 := $this;
+    assert { :sourceloc "/Users/schaef/git/jar2bpl/jar2bpl_test/regression/corner_cases/cc01/CornerCases01.java",5,-1,-1,-1 } true;
+    call $exception := void$java.lang.Object$$la$init$ra$$38(this36);
+    assert { :sourceloc "/Users/schaef/git/jar2bpl/jar2bpl_test/regression/corner_cases/cc01/CornerCases01.java",5,-1,-1,-1 } true;
     return;
 }
 
